Substitution

theories/Substitution.v
@@ -3,6 +3,11 @@
 From MailboxTypes Require Export Environment.
 From MailboxTypes Require Export Syntax.
 From MailboxTypes Require Import Util.
+From MailboxTypes Require Import TypingRules.
+
+
+(** We assume functional extensionality in order to proof statements about substitutions. *)
+From Stdlib Require Import FunctionalExtensionality.
 
 Generalizable All Variables.
 
@@ -24,15 +29,15 @@ Section subs_def.
   *)
 
   (** The identity renaming just returns its argument *)
-  Definition id (v : nat) := v.
+  Definition id {X} (x : X) := x.
 
   (** Shifting is a renaming that increments a variable by one *)
   Definition shift := S.
 
   (** Extension extends a substitution sigma : nat -> Term with a new element *)
-  Definition extend (v : nat) (xi : nat -> nat) :=
+  Definition extend {X : Type} (x : X) (xi : nat -> X) :=
     fun n => match n with
-             | 0 => v
+             | 0 => x
              | S n => xi n
              end.
 
@@ -46,15 +51,170 @@ Section subs_def.
     | _ => v
     end.
 
-  Fixpoint rename_Term (xi : nat -> nat) (t : Term) : Term :=
-    match t with
-    | TValue v => TValue (rename_Value xi v)
-    | TLet t1 t2 => TLet (rename_Term xi t1) (rename_Term (lift_renaming xi) t2)
-    | TApp def values => TApp def values
-    | _ => t
+  Definition lift_Value (sigma : nat -> Value) : nat -> Value :=
+    extend (ValueVar (Var 0)) (sigma >> (rename_Value shift)).
+
+  Definition subst_Value (sigma_term : nat -> Value) (v : Value) : Value :=
+    match v with
+    | ValueVar (Var x) => sigma_term x
+    | v => v
     end.
-  
-  Definition up_Term_Term (sigma : nat -> Term) : nat -> Term :=
-    extend () (funcomp () sigma).
-  Definition subst_Term (sigma_term : nat -> Term) (t : Term) := t.
+
+  Fixpoint subst_Term (sigma : nat -> Value) (t : Term) : Term :=
+    match t with
+    | TValue v => TValue (subst_Value sigma v)
+    | TLet t1 t2  => TLet (subst_Term sigma t1) (subst_Term (lift_Value sigma) t2)
+    | TApp def v => TApp def (subst_Value sigma v)
+    | TSpawn t1 => TSpawn (subst_Term sigma t1)
+    | TNew => TNew
+    | TSend v m v' => TSend (subst_Value sigma v) m (subst_Value sigma v')
+    | TGuard v e guards => TGuard (subst_Value sigma v) e (map (subst_Guard sigma) guards)
+    end
+  with subst_Guard (sigma : nat -> Value) (g : Guard) : Guard :=
+    match g with
+    | GFail => GFail
+    | GFree t1 => GFree (subst_Term sigma t1)
+    (* We lift sigma twice, because a receive introduces 2 new variables *)
+    | GReceive m t1 => GReceive m (subst_Term (lift_Value (lift_Value sigma)) t1)
+    end.
+
+  Definition nVar n := ValueVar (Var n).
+
+  Definition subst_1 (t : Term) (v : Value) : Term :=
+    subst_Term (extend v nVar) t.
+
+  Notation "s .: sigma" := (extend s sigma) (at level 70).
+  Notation "s [ sigma ]" := (subst_Term sigma s) (at level 7, left associativity, format "s '/' [ sigma ]").
+  Notation "s '..'" := (extend s nVar) (at level 1, format "s ..").
+
+  Definition subst_tTest (t : Term) (v : Value) : Term :=
+    t[v..].
+
+  (*Compute (subst_1 (TValue (ValueVar (Var 0))) ValueUnit ).*)
+  (*Compute ((TValue (ValueVar (Var 0)))[ValueUnit..]).*)
+
+  Lemma subst_1_Var_0 : forall v, subst_1 (TValue (ValueVar (Var 0))) v = TValue v.
+  Proof.
+    destruct v; unfold subst_1; reflexivity.
+  Qed.
+
+  Lemma subst_id_left : forall {T U} (f : T -> U), id >> f = f.
+  Proof.
+    intros; reflexivity.
+  Qed.
+
+  Lemma subst_id_right : forall {T U} (f : T -> U), f = id >> f.
+  Proof.
+    intros; reflexivity.
+  Qed.
+
+  Lemma extend_distr : forall {T U} (s : T) (sigma : nat -> T) (f : T -> U),
+    (extend s sigma) >> f = extend (f s) (sigma >> f).
+  Proof.
+    (* Extensionality is required to prove this *)
+    intros; extensionality x; now destruct x.
+  Qed.
+
+  Lemma interaction : forall {T} (s : T) (sigma : nat -> T),
+    shift >> (extend s sigma) = sigma.
+  Proof.
+    reflexivity.
+  Qed.
+
+  Lemma eta_id : extend 0 shift = id.
+  Proof.
+    (* Extensionality is required to prove this *)
+    intros; extensionality x; now destruct x.
+  Qed.
+
+  Lemma eta_extend : forall {T} (sigma : nat -> T),
+    extend (sigma 0) (shift >> sigma) = sigma.
+  Proof.
+    (* Extensionality is required to prove this *)
+    intros; extensionality x; now destruct x.
+  Qed.
+
+  Lemma lift_Value_id : lift_Value nVar = nVar.
+  Proof.
+    extensionality x.
+    intros; now destruct x.
+  Qed.
+
+  Lemma subst_Value_id : forall v, subst_Value nVar v = v.
+  Proof.
+    destruct v; try reflexivity; now destruct v.
+  Qed.
+
+  Lemma subst_id: forall t,
+    subst_Term nVar t = t.
+  Proof.
+    intros t.
+    induction t using @Term_ind2 with (PG := fun g => subst_Guard nVar g = g); simpl;
+    try (now repeat rewrite subst_Value_id);
+    try (now rewrite IHt).
+    - rewrite IHt1; rewrite lift_Value_id; now rewrite IHt2.
+    - induction gs as [| g gs]; rewrite subst_Value_id.
+      + reflexivity.
+      + inversion H as [| ? ? Eq F]; subst.
+        apply IHgs in F; injection F.
+        simpl; intros -> ?; now rewrite Eq.
+    - repeat rewrite lift_Value_id; now rewrite IHt.
+  Qed.
+
+  Lemma sub_lemma : forall p env1 env2 env A A' B v t,
+    WellTypedTerm p (Some A :: env1) t B ->
+    WellTypedTerm p env2 (TValue v) A' ->
+    A' ≤ A ->
+    (None :: env1) +ₑ env2 ~= env ->
+    WellTypedTerm p env (t[v..]) B.
+  Proof.
+    (*intros * WT1 WT2 Sub Dis.*)
+    (*remember (Some A :: env1) as env1' eqn:E.*)
+    (*generalize dependent env1.*)
+    (*induction WT1 using @WellTypedTerm_ind3 with*)
+    (*  (P0 := fun _ _ _ _ => True)*)
+    (*  (P1 := fun _ _ _ _ => True).*)
+    (*intros * WT1.*)
+    (*revert env2 env v A'.*)
+    (*remember (Some A :: env1) as env1' eqn:E.*)
+    (*generalize dependent A.*)
+    (*generalize dependent env1.*)
+    (*induction WT1; intros.*)
+    (*- simpl in *.*)
+    (*  assert (zero : v = 0). admit.*)
+    (*  assert (SubTy : T = A). admit.*)
+    (*  subst. simpl.*)
+    (*  (*rewrite subst_1_Var_0.*)*)
+    (*  eapply SUB with (env2 := env2).*)
+    (*  (* env1 is empty, thus env2 = env *)*)
+    (*  admit.*)
+    (*  apply H2.*)
+    (*  apply H1.*)
+    (*- inversion H; subst; discriminate.*)
+    (*- inversion H; subst; discriminate.*)
+    (*- inversion H; subst; discriminate.*)
+    (*- eapply APP.*)
+    (*  + apply H.*)
+    (*  + eapply IHWT1. apply E. apply H0. assumption. assumption.*)
+    (*- subst.*)
+    (*  inversion H; subst.*)
+    (*  + eapply LET.*)
+    (*    * apply (EnvironmentDis_implies_Comb _ _ _ H2).*)
+    (*    * eapply IHWT1_1.*)
+    (*      -- reflexivity.*)
+    (*      -- apply H0.*)
+    (*      -- assumption.*)
+    (*      -- admit.*)
+    (*- admit.*)
+    (*- subst; inversion H; subst; discriminate.*)
+    (*- admit.*)
+    (*- admit.*)
+    (*- subst. inversion H3; subst; inversion H; subst.*)
+    (*  + eapply SUB.*)
+    (*    * apply EnvSubtypeRefl.*)
+    (*    * apply H0.*)
+    (*    * eapply IHWT1.*)
+    (*      -- *)
+    Admitted.
+
 End subs_def.
