theories/Types_intrinsic.v
@@ -23,113 +23,38 @@ Inductive Member : TUsage -> Env -> Prop :=
 (*lookup {Γ , A} {zero} (s≤s z≤n) = A*)
 (*lookup {Γ , A} {suc n} (s≤s p) = lookup p*)
 
-Inductive Term' (prog : Prog) : Env -> TUsage -> Prop :=
-  | VAR : forall env T, Member T env -> Term' prog env T
-  | APP : forall env envList vList definition bodyType argumentTypes term,
-      definitions prog definition = (FunDef definition argumentTypes bodyType term) ->
-      [ envList ]+ₑ ~= env ->
-      Forall3 (Term' prog) envList (map TValue vList) (argumentTypes) ->
-      Term' prog env (TApp definition vList) bodyType
-.
-
-Inductive WellTypedTerm (prog : Prog) : Env -> Term -> TUsage -> Prop :=
-  (* Var *)
-  | VAR   : forall v env T,
-      SingletonEnv env ->
-      lookup v env = Some T ->
-      WellTypedTerm prog env (TValue (ValueVar (Var v))) T
-  (* Consts *)
-  | TRUE  : forall env,
-      EmptyEnv env ->
-      WellTypedTerm prog env (TValue (ValueBool true)) (TUBase BTBool)
-  | FALSE : forall env,
-      EmptyEnv env ->
-      WellTypedTerm prog env (TValue (ValueBool false)) (TUBase BTBool)
-  | UNIT  : forall env,
-      EmptyEnv env ->
-      WellTypedTerm prog env (TValue ValueUnit) (TUBase BTUnit)
-  (* App *)
-  | APP : forall env envList vList definition bodyType argumentTypes term,
-      definitions prog definition = (FunDef definition argumentTypes bodyType term) ->
-      [ envList ]+ₑ ~= env ->
-      Forall3 (WellTypedTerm prog) envList (map TValue vList) (argumentTypes) ->
-      WellTypedTerm prog env (TApp definition vList) bodyType
-  (* Let *)
-  | LET   : forall env env1 env2 T1 T2 t1 t2, 
+Inductive Term' (prog : Prog) (env : Env) : TUsage -> Prop :=
+  | VAR : forall T, Member T env -> Term' prog env T
+  (*| APP : forall v definition bodyType argumentType term,*)
+  (*    definitions prog definition = (FunDef definition argumentType bodyType term) ->*)
+  (*    Term' prog env (TValue v) argumentType ->*)
+  (*    Term' prog env (TApp definition v) bodyType*)
+  | LET : forall env1 env2 T1 T2,
       env1 ▷ₑ env2 ~= env ->
-      WellTypedTerm prog env1 t1 ⌊ T1 ⌋ ->
-      WellTypedTerm prog (Some ⌊ T1 ⌋ :: env2) t2 T2 ->
-      WellTypedTerm prog env (TLet t1 t2) T2
-  (* Spawn *)
-  | SPAWN : forall env t,
-      WellTypedTerm prog env t (TUBase BTUnit) ->
-      WellTypedTerm prog ⌈ env ⌉ₑ (TSpawn t) (TUBase BTUnit)
-  (* New *)
-  | NEW : forall env,
-      EmptyEnv env ->
-      WellTypedTerm prog env TNew (? 𝟙 ^^ •)
-  (* Send *)
-  (* TODO: Maybe try a recursive approach with this rule *)
-  | SEND : forall env env' envList tList vList m v,
-      WellTypedTerm prog env' (TValue v) (! « m » ^^ ◦) ->
-      signature prog m = tList ->
-      [ (env' :: envList) ]+ₑ ~= env ->
-      Forall3 (WellTypedTerm prog) envList (map TValue vList) (map secondType tList) ->
-      WellTypedTerm prog env (TSend v m vList) (TUBase BTUnit)
-  (* Guard *)
-  | GUARD : forall env env1 env2 guards v T e f,
-      env1 +ₑ env2 ~= env ->
-      WellTypedTerm prog env1 (TValue v) (? f ^^ •) ->
-      WellTypedGuards prog env2 guards T f ->
-      e ⊑ f ->
-      f ⊧ f ->
-      WellTypedTerm prog env (TGuard v e guards) T
-  (* Sub *)
-  | SUB : forall t env1 env2 T1 T2,
-      env1 ≤ₑ env2 ->
+      Term' prog env1 ⌊ T1 ⌋ ->
+      Term' prog (Some ⌊ T1 ⌋ :: env2) T2 ->
+      Term' prog env T2
+  | NEW : EmptyEnv env -> Term' prog env (? 𝟙 ^^ •)
+  | SUB : forall env' T1 T2,
+      env ≤ₑ env' ->
       T1 ≤ T2 ->
-      WellTypedTerm prog env2 t T1 ->
-      WellTypedTerm prog env1 t T2
-with WellTypedGuards (prog : Prog) : Env -> list Guard -> TUsage -> MPattern -> Prop :=
-  | SINGLE : forall T e env g,
-      WellTypedGuard prog env g T e ->
-      WellTypedGuards prog env (g :: nil) T e
-  | SEQ : forall T e es env guards g,
-      WellTypedGuard prog env g T e ->
-      WellTypedGuards prog env guards T es ->
-      WellTypedGuards prog env (g :: guards) T (e ⊕ es)
-with WellTypedGuard (prog : Prog) : Env -> Guard -> TUsage -> MPattern -> Prop :=
-  (* Fail *)
-  | FAIL : forall t env, WellTypedGuard prog env GFail t 𝟘
-  (* Free *)
-  | FREE : forall t env T,
-      WellTypedTerm prog env t T ->
-      WellTypedGuard prog env (GFree t) T 𝟙
-  (* Receive *)
-  | RECEIVE : forall t m env T tList e mailbox,
-      signature prog m = tList ->
-      BaseTypes tList \/ BaseEnv env ->
-      WellTypedTerm prog ((toEnv (map secondType tList)) ++ [Some (? e ^^ •)] ++ env) t T ->
-      WellTypedGuard prog env (GReceive m mailbox t) T (« m » ⊙ e).
-
-Inductive WellTypedDefinition (prog : Prog) : FunctionDefinition -> Prop :=
-  | FUNDEF : forall defName argumentTypes body bodyType,
-      WellTypedTerm prog (toEnv argumentTypes) body bodyType ->
-      WellTypedDefinition prog (FunDef defName argumentTypes bodyType body).
-
-Inductive WellTypedProgram (prog : Prog) : Prop :=
-  PROG :
-    (forall def, WellTypedDefinition prog (definitions prog def)) ->
-    WellTypedTerm prog nil (initialTerm prog) (TUBase BTUnit) -> WellTypedProgram prog.
+      Term' prog env' T1 ->
+      Term' prog env T2
+with Guards' (prog : Prog) (env : Env) : TUsage -> MPattern -> Prop :=
+  | SINGLE : forall T e,
+      Guard' prog env T e ->
+      Guards' prog env T e
+  | SEQ : forall T e es,
+      Guard' prog env T e ->
+      Guards' prog env T es ->
+      Guards' prog env T (e ⊕ es)
+with Guard' (prog : Prog) (env : Env) : TUsage -> MPattern -> Prop :=
+  | FAIL : forall T, Guard' prog env T 𝟘
+  | FREE : forall T, Term' prog env T -> Guard' prog env T 𝟙
+  | RECEIVE : forall m T T' e,
+      signature prog m = T' ->
+      BaseType T' \/ BaseEnv env ->
+      Term' prog (Some (secondType T') :: Some (? e ^^ •) :: env) T ->
+      Guard' prog env T (« m » ⊙ e).
 
 End typing_rules_def.
-
-Section well_typed_def.
-
-Generalizable All Variables.
-Context `{M : IMessage Message}.
-Context `{D : IDefinitionName DefinitionName}.
-
-(*Definition EnvEqFV {T : TUsage} (p: Prog) (env : Env) (m : Term) : WellTypedTerm p env m T -> Prop.*)
-
-End well_typed_def.
