theories/test.v
@@ -1,0 +1,87 @@
+Inductive WellTypedTerm (prog : Prog) : Env -> Term -> TUsage -> Prop :=
+  (* Var *)
+| VAR   : forall v env T,
+      SingletonEnv env ->
+      lookup v env = Some T ->
+      WellTypedTerm prog env (TValue (ValueVar (Var v))) T
+  (* Consts *)
+  | TRUE  : forall env,
+      EmptyEnv env ->
+      WellTypedTerm prog env (TValue (ValueBool true)) (TUBase BTBool)
+  | FALSE : forall env,
+      EmptyEnv env ->
+      WellTypedTerm prog env (TValue (ValueBool false)) (TUBase BTBool)
+  | UNIT  : forall env,
+      EmptyEnv env ->
+      WellTypedTerm prog env (TValue ValueUnit) (TUBase BTUnit)
+  (* App *)
+  | APP : forall env v definition bodyType argumentType term,
+      definitions prog definition = (FunDef definition argumentType bodyType term) ->
+      WellTypedTerm prog env (TValue v) argumentType ->
+      WellTypedTerm prog env (TApp definition v) bodyType
+  (* Let *)
+  | LET   : forall env env1 env2 T1 T2 t1 t2, 
+      env1 ▷ₑ env2 ~= env ->
+      WellTypedTerm prog env1 t1 ⌊ T1 ⌋ ->
+      WellTypedTerm prog (Some ⌊ T1 ⌋ :: env2) t2 T2 ->
+      WellTypedTerm prog env (TLet t1 t2) T2
+  (* Spawn *)
+  | SPAWN : forall env t,
+      WellTypedTerm prog env t (TUBase BTUnit) ->
+      WellTypedTerm prog ⌈ env ⌉ₑ (TSpawn t) (TUBase BTUnit)
+  (* New *)
+  | NEW : forall env,
+      EmptyEnv env ->
+      WellTypedTerm prog env TNew (? 𝟙 ^^ •)
+  (* Send *)
+  | SEND : forall env env1 env2 T m v1 v2,
+      WellTypedTerm prog env1 (TValue v1) (! « m » ^^ ◦) ->
+      signature prog m = T ->
+      env1 +ₑ env2 ~= env ->
+      WellTypedTerm prog env2 (TValue v2) ⌈ T ⌉ ->
+      WellTypedTerm prog env (TSend v1 m v2) (TUBase BTUnit)
+  (* Guard *)
+  | GUARD : forall env env1 env2 guards v T e f,
+      env1 +ₑ env2 ~= env ->
+      WellTypedTerm prog env1 (TValue v) (? f ^^ •) ->
+      WellTypedGuards prog env2 guards T f ->
+      e ⊑ f ->
+      f ⊧ f ->
+      WellTypedTerm prog env (TGuard v e guards) T
+  (* Sub *)
+  | SUB : forall t env1 env2 T1 T2,
+      env1 ≤ₑ env2 ->
+      T1 ≤ T2 ->
+      WellTypedTerm prog env2 t T1 ->
+      WellTypedTerm prog env1 t T2
+with WellTypedGuards (prog : Prog) : Env -> list Guard -> TUsage -> MPattern -> Prop :=
+  | SINGLE : forall T e env g,
+      WellTypedGuard prog env g T e ->
+      WellTypedGuards prog env (g :: nil) T e
+  | SEQ : forall T e es env guards g,
+      WellTypedGuard prog env g T e ->
+      WellTypedGuards prog env guards T es ->
+      WellTypedGuards prog env (g :: guards) T (e ⊕ es)
+with WellTypedGuard (prog : Prog) : Env -> Guard -> TUsage -> MPattern -> Prop :=
+  (* Fail *)
+  | FAIL : forall t env, WellTypedGuard prog env GFail t 𝟘
+  (* Free *)
+  | FREE : forall t env T,
+      WellTypedTerm prog env t T ->
+      WellTypedGuard prog env (GFree t) T 𝟙
+  (* Receive *)
+  | RECEIVE : forall t m env BT T e,
+      signature prog m = BT ->
+      BaseType BT \/ BaseEnv env ->
+      WellTypedTerm prog (Some ⌈ BT ⌉ :: Some (? e ^^ •) :: env) t T ->
+      WellTypedGuard prog env (GReceive m t) T (« m » ⊙ e).
+
+Inductive WellTypedDefinition (prog : Prog) : FunctionDefinition -> Prop :=
+  | FUNDEF : forall defName argumentType body bodyType,
+      WellTypedTerm prog [Some argumentType] body bodyType ->
+      WellTypedDefinition prog (FunDef defName argumentType bodyType body).
+
+Inductive WellTypedProgram (prog : Prog) : Prop :=
+  PROG :
+    (forall def, WellTypedDefinition prog (definitions prog def)) ->
+    WellTypedTerm prog nil (initialTerm prog) (TUBase BTUnit) -> WellTypedProgram prog.
